coq/scripts/contracts_generate.sh
@@ -9,6 +9,8 @@ set -x #echo on
 # erc20
 ../build/solc/solc --ir-coq --optimize CoqOfSolidity/contracts/erc20/erc20.sol \
   > CoqOfSolidity/contracts/erc20/erc20.v
+../build/solc/solc --ir-optimized --optimize CoqOfSolidity/contracts/erc20/erc20.sol \
+  > CoqOfSolidity/contracts/erc20/erc20.yul
 ../build/solc/solc --ir-optimized-ast-json --optimize CoqOfSolidity/contracts/erc20/erc20.sol \
   | tail -1 \
   | jq 'walk(if type == "object" then del(.nativeSrc, .src, .type) else . end)' \
@@ -21,6 +23,8 @@ python scripts/shallow_embed_proof.py CoqOfSolidity/contracts/erc20/erc20.json \
 # SCL_mulmuladdX_fullgen_b4
 ../build/solc/solc --ir-coq --optimize CoqOfSolidity/contracts/scl/mulmuladdX_fullgen_b4/contract.sol \
   > CoqOfSolidity/contracts/scl/mulmuladdX_fullgen_b4/contract.v
+../build/solc/solc --ir-optimized --optimize CoqOfSolidity/contracts/scl/mulmuladdX_fullgen_b4/contract.sol \
+  > CoqOfSolidity/contracts/scl/mulmuladdX_fullgen_b4/contract.yul
 ../build/solc/solc --ir-optimized-ast-json --optimize CoqOfSolidity/contracts/scl/mulmuladdX_fullgen_b4/contract.sol \
   | tail -1 \
   | jq 'walk(if type == "object" then del(.nativeSrc, .src, .type) else . end)' \
